AwsCryptographicMaterialProviders/runtimes/java/src/main/smithy-generated/software/amazon/cryptography/materialProviders/model/CreateAwsKmsRsaKeyringInput.java
@@ -1,0 +1,160 @@
+// Copyright Amazon.com Inc. or its affiliates. All Rights Reserved.
+// SPDX-License-Identifier: Apache-2.0
+// Do not modify this file. This file is machine generated, and any changes to it will be overwritten.
+package software.amazon.cryptography.materialProviders.model;
+
+import com.amazonaws.services.kms.AWSKMS;
+import com.amazonaws.services.kms.model.EncryptionAlgorithmSpec;
+import java.nio.ByteBuffer;
+import java.util.List;
+import java.util.Objects;
+
+public class CreateAwsKmsRsaKeyringInput {
+  private final ByteBuffer publicKey;
+
+  private final String kmsKeyId;
+
+  private final EncryptionAlgorithmSpec encryptionAlgorithm;
+
+  private final AWSKMS kmsClient;
+
+  private final List<String> grantTokens;
+
+  protected CreateAwsKmsRsaKeyringInput(BuilderImpl builder) {
+    this.publicKey = builder.publicKey();
+    this.kmsKeyId = builder.kmsKeyId();
+    this.encryptionAlgorithm = builder.encryptionAlgorithm();
+    this.kmsClient = builder.kmsClient();
+    this.grantTokens = builder.grantTokens();
+  }
+
+  public ByteBuffer publicKey() {
+    return this.publicKey;
+  }
+
+  public String kmsKeyId() {
+    return this.kmsKeyId;
+  }
+
+  public EncryptionAlgorithmSpec encryptionAlgorithm() {
+    return this.encryptionAlgorithm;
+  }
+
+  public AWSKMS kmsClient() {
+    return this.kmsClient;
+  }
+
+  public List<String> grantTokens() {
+    return this.grantTokens;
+  }
+
+  public Builder toBuilder() {
+    return new BuilderImpl(this);
+  }
+
+  public static Builder builder() {
+    return new BuilderImpl();
+  }
+
+  public interface Builder {
+    Builder publicKey(ByteBuffer publicKey);
+
+    ByteBuffer publicKey();
+
+    Builder kmsKeyId(String kmsKeyId);
+
+    String kmsKeyId();
+
+    Builder encryptionAlgorithm(EncryptionAlgorithmSpec encryptionAlgorithm);
+
+    EncryptionAlgorithmSpec encryptionAlgorithm();
+
+    Builder kmsClient(AWSKMS kmsClient);
+
+    AWSKMS kmsClient();
+
+    Builder grantTokens(List<String> grantTokens);
+
+    List<String> grantTokens();
+
+    CreateAwsKmsRsaKeyringInput build();
+  }
+
+  static class BuilderImpl implements Builder {
+    protected ByteBuffer publicKey;
+
+    protected String kmsKeyId;
+
+    protected EncryptionAlgorithmSpec encryptionAlgorithm;
+
+    protected AWSKMS kmsClient;
+
+    protected List<String> grantTokens;
+
+    protected BuilderImpl() {
+    }
+
+    protected BuilderImpl(CreateAwsKmsRsaKeyringInput model) {
+      this.publicKey = model.publicKey();
+      this.kmsKeyId = model.kmsKeyId();
+      this.encryptionAlgorithm = model.encryptionAlgorithm();
+      this.kmsClient = model.kmsClient();
+      this.grantTokens = model.grantTokens();
+    }
+
+    public Builder publicKey(ByteBuffer publicKey) {
+      this.publicKey = publicKey;
+      return this;
+    }
+
+    public ByteBuffer publicKey() {
+      return this.publicKey;
+    }
+
+    public Builder kmsKeyId(String kmsKeyId) {
+      this.kmsKeyId = kmsKeyId;
+      return this;
+    }
+
+    public String kmsKeyId() {
+      return this.kmsKeyId;
+    }
+
+    public Builder encryptionAlgorithm(EncryptionAlgorithmSpec encryptionAlgorithm) {
+      this.encryptionAlgorithm = encryptionAlgorithm;
+      return this;
+    }
+
+    public EncryptionAlgorithmSpec encryptionAlgorithm() {
+      return this.encryptionAlgorithm;
+    }
+
+    public Builder kmsClient(AWSKMS kmsClient) {
+      this.kmsClient = kmsClient;
+      return this;
+    }
+
+    public AWSKMS kmsClient() {
+      return this.kmsClient;
+    }
+
+    public Builder grantTokens(List<String> grantTokens) {
+      this.grantTokens = grantTokens;
+      return this;
+    }
+
+    public List<String> grantTokens() {
+      return this.grantTokens;
+    }
+
+    public CreateAwsKmsRsaKeyringInput build() {
+      if (Objects.isNull(this.kmsKeyId()))  {
+        throw new IllegalArgumentException("Missing value for required field `kmsKeyId`");
+      }
+      if (Objects.isNull(this.encryptionAlgorithm()))  {
+        throw new IllegalArgumentException("Missing value for required field `encryptionAlgorithm`");
+      }
+      return new CreateAwsKmsRsaKeyringInput(this);
+    }
+  }
+}
