AwsCryptographicMaterialProviders/test/Keyrings/AwsKms/TestAwsKmsRsaKeyring.dfy
@@ -1,0 +1,68 @@
+// Copyright Amazon.com Inc. or its affiliates. All Rights Reserved.
+// SPDX-License-Identifier: Apache-2.0
+
+include "../../../src/Index.dfy"
+include "../../../src/Keyrings/AwsKms/AwsKmsDiscoveryKeyring.dfy"
+include "../../TestUtils.dfy"
+include "../../../../ComAmazonawsKms/src/Index.dfy"
+
+module TestAwsKmsRsaKeyring {
+  import opened Wrappers
+   import opened UInt = StandardLibrary.UInt
+  import MaterialProviders
+  import Types = AwsCryptographyMaterialProvidersTypes
+  import AwsKmsRsaKeyring
+  import TestUtils
+  import ComAmazonawsKmsTypes
+
+  // Smoke tests for valid configurations
+  // TODO These should eventually be covered by formal verification
+
+  method {:test} TestValidEncryptOnlyConfiguration() {
+    var mpl :- expect MaterialProviders.MaterialProviders();
+
+    var publicKey: seq<uint8> := []; // TODO for now empty bytestring is accepted
+
+    var result :- expect mpl.CreateAwsKmsRsaKeyring(Types.CreateAwsKmsRsaKeyringInput(
+        publicKey := Some(publicKey),
+        kmsKeyId := TestUtils.SHARED_TEST_KEY_ARN,
+        encryptionAlgorithm := ComAmazonawsKmsTypes.EncryptionAlgorithmSpec.RSAES_OAEP_SHA_1,
+        kmsClient := None(),
+        grantTokens := None()
+    ));
+  }
+
+  method {:test} TestValidDecryptOnlyConfiguration() {
+    var mpl :- expect MaterialProviders.MaterialProviders();
+
+    // TODO awkward way to initialize a KMS client
+    var clientSupplier :- expect mpl.CreateDefaultClientSupplier(Types.CreateDefaultClientSupplierInput());
+    var kmsClient :- expect clientSupplier.GetClient(Types.GetClientInput(region:="us-west-2"));
+
+    var result :- expect mpl.CreateAwsKmsRsaKeyring(Types.CreateAwsKmsRsaKeyringInput(
+        publicKey := None(),
+        kmsKeyId := TestUtils.SHARED_TEST_KEY_ARN,
+        encryptionAlgorithm := ComAmazonawsKmsTypes.EncryptionAlgorithmSpec.RSAES_OAEP_SHA_1,
+        kmsClient := Some(kmsClient),
+        grantTokens := None()
+    ));
+  }
+
+  method {:test} TestValidEncryptDecryptConfiguration() {
+    var mpl :- expect MaterialProviders.MaterialProviders();
+
+    var publicKey: seq<uint8> := []; // TODO for now empty bytestring is accepted
+
+    // TODO awkward way to initialize a KMS client
+    var clientSupplier :- expect mpl.CreateDefaultClientSupplier(Types.CreateDefaultClientSupplierInput());
+    var kmsClient :- expect clientSupplier.GetClient(Types.GetClientInput(region:="us-west-2"));
+
+    var result :- expect mpl.CreateAwsKmsRsaKeyring(Types.CreateAwsKmsRsaKeyringInput(
+        publicKey := Some(publicKey),
+        kmsKeyId := TestUtils.SHARED_TEST_KEY_ARN,
+        encryptionAlgorithm := ComAmazonawsKmsTypes.EncryptionAlgorithmSpec.RSAES_OAEP_SHA_1,
+        kmsClient := Some(kmsClient),
+        grantTokens := None()
+    ));
+  }
+}
